Add Config. Fixed PrintOrder bug. Updated Coq Spec (added laws, defined instances)

src/edu/virginia/cs/DBTrademaker.scala
@@ -1,10 +1,8 @@
 package edu.virginia.cs
 
 import edu.virginia.cs.Framework._
-import edu.virginia.cs.Framework.DBSpecification
-import edu.virginia.cs.Framework.DBImplementation
-import edu.virginia.cs.Framework.DBBenchmark
-import edu.virginia.cs.Framework.DBBenchmarkResult
+import edu.virginia.cs.Framework.Types.DBSpecification
+import edu.virginia.cs.Framework.Types.DBImplementation
 import edu.mit.csail.sdg.alloy4.A4Reporter
 import edu.mit.csail.sdg.alloy4.Err
 import edu.mit.csail.sdg.alloy4.ErrorWarning
@@ -18,89 +16,110 @@ import edu.mit.csail.sdg.alloy4compiler.translator.TranslateAlloyToKodkod
 import java.io.IOException
 import java.io.File
 import edu.virginia.cs.Synthesizer.SmartBridge
-import edu.virginia.cs.Analyzer.DBRunBenchmark
-import edu.virginia.cs.Synthesizer.FileOperation
 import edu.virginia.cs.Synthesizer.AlloyOMToAlloyDM
 import java.util.HashMap
 import java.util.ArrayList
 import edu.virginia.cs.Synthesizer.CodeNamePair
 import edu.virginia.cs.Synthesizer.Sig
-import edu.virginia.cs.Synthesizer.ORMParser
-import edu.virginia.cs.Synthesizer.Types.ObjectSpec
-import edu.virginia.cs.Synthesizer.Types.ObjectSet
+import edu.virginia.cs.Framework.Types.ObjectSpec
+import edu.virginia.cs.Framework.Types.ObjectSet
 import java.io.FileOutputStream
 import java.io.PrintWriter
 import edu.virginia.cs.Synthesizer.LoadSynthesizer
-import edu.virginia.cs.Synthesizer.Types.ObjectOfDM
-import edu.virginia.cs.Synthesizer.Types.AbstractLoad
-import edu.virginia.cs.Synthesizer.Types.AbstractQuery
-import edu.virginia.cs.Synthesizer.Types.AbstractQuery.Action
-import edu.virginia.cs.Synthesizer.Types.ConcreteQuery
-import edu.virginia.cs.Synthesizer.Types.SpecializedQuery
-import edu.virginia.cs.Synthesizer.Types.ConcreteLoad
-import edu.virginia.cs.Synthesizer.SolveAlloyDM
-import edu.virginia.cs.Synthesizer.Types.FormalAbstractLoadSet
-import edu.virginia.cs.Synthesizer.Types.DBFormalAbstractMeasurementFunctionSet
-import edu.virginia.cs.Framework.DBFormalImplementation
-import edu.virginia.cs.Synthesizer.Types.DBFormalConcreteMeasurementFunctionSet
+import edu.virginia.cs.Framework.Types.ObjectOfDM
+import edu.virginia.cs.Framework.Types.AbstractLoad
+import edu.virginia.cs.Framework.Types.AbstractQuery
+import edu.virginia.cs.Framework.Types.ConcreteQuery
+import edu.virginia.cs.Framework.Types.SpecializedQuery
+import edu.virginia.cs.Framework.Types.ConcreteLoad
+import edu.virginia.cs.Framework.Types.FormalAbstractLoadSet
+import edu.virginia.cs.Framework.Types.DBFormalAbstractMeasurementFunctionSet
+import edu.virginia.cs.Framework.Types.DBFormalImplementation
+import edu.virginia.cs.Framework.Types.DBFormalConcreteMeasurementFunctionSet
 import scala.collection.JavaConversions._
 import java.text.NumberFormat
 import java.text.ParsePosition
 import edu.virginia.cs.Synthesizer.PrintOrder
-import edu.virginia.cs.Synthesizer.Types.DBFormalAbstractMeasurementFunction
-import edu.virginia.cs.Synthesizer.Types.DBFormalConcreteTimeMeasurementFunction
-import edu.virginia.cs.Synthesizer.Types.DBFormalConcreteSpaceMeasurementFunction
-import edu.virginia.cs.Synthesizer.Types.DBFormalAbstractTimeMeasurementFunction
-import edu.virginia.cs.Synthesizer.Types.DBFormalAbstractSpaceMeasurementFunction
+import edu.virginia.cs.Framework.Types.DBFormalAbstractMeasurementFunction
+import edu.virginia.cs.Framework.Types.DBFormalConcreteTimeMeasurementFunction
+import edu.virginia.cs.Framework.Types.DBFormalConcreteSpaceMeasurementFunction
+import edu.virginia.cs.Framework.Types.DBFormalAbstractTimeMeasurementFunction
+import edu.virginia.cs.Framework.Types.DBFormalAbstractSpaceMeasurementFunction
 import java.io.FileNotFoundException
 import scala.sys.process._
-import edu.virginia.cs.Synthesizer.Types.DBConcreteMeasurementFunctionSet
-import edu.virginia.cs.Synthesizer.Types.DBConcreteMeasurementFunction
-import edu.virginia.cs.Synthesizer.Types.DBConcreteTimeMeasurementFunction
-import edu.virginia.cs.Synthesizer.Types.DBConcreteSpaceMeasurementFunction
-import edu.virginia.cs.Synthesizer.Types.DBMeasurementResult
+import edu.virginia.cs.Framework.Types.DBConcreteMeasurementFunctionSet
+import edu.virginia.cs.Framework.Types.DBConcreteMeasurementFunction
+import edu.virginia.cs.Framework.Types.DBConcreteTimeMeasurementFunction
+import edu.virginia.cs.Framework.Types.DBConcreteSpaceMeasurementFunction
+import edu.virginia.cs.Framework.Types.DBMeasurementResult
+import edu.virginia.cs.Synthesizer.ORMParser
+import edu.virginia.cs.Synthesizer.FileOperation
+import edu.virginia.cs.Framework.Types.DBFormalSpecification
+import edu.virginia.cs.Framework.Types.AbstractQuery.Action
+import edu.virginia.cs.Framework.Types.DBSpaceMeasurementResult
+import edu.virginia.cs.Framework.Types.DBTimeMeasurementResult
 
 class DBTrademaker extends TrademakerFramework {
 
-  var solveDM: SolveAlloyDM = null
+  var isDebugOn = AppConfig.getDebug
 
-  var schemas = new HashMap[String, HashMap[String, ArrayList[CodeNamePair[String]]]]()
-  var parents = new HashMap[String, ArrayList[CodeNamePair[String]]]()
-  var reverseTAss = new HashMap[String, ArrayList[CodeNamePair[String]]]()
-  var foreignKeys = new HashMap[String, ArrayList[CodeNamePair[String]]]()
-  var association = new HashMap[String, HashMap[String, CodeNamePair[String]]]()
-  var primaryKeys = new HashMap[String, ArrayList[CodeNamePair[String]]]()
-  var fields = new HashMap[String, ArrayList[CodeNamePair[String]]]()
-  var fieldsTable = new HashMap[String, ArrayList[CodeNamePair[String]]]()
-  var allFields = new HashMap[String, ArrayList[String]]()
-  var fieldType = new HashMap[String, ArrayList[CodeNamePair[String]]]()
-
-  /**
-   *     parents.put(fImpFileName, parser.getParents());
-   * reverseTAss.put(fImpFileName, parser.getReverseTAssociate());
-   * foreignKeys.put(fImpFileName, parser.getForeignKey());
-   * association.put(fImpFileName, parser.getAssociation());
-   * primaryKeys.put(fImpFileName, parser.getPrimaryKeys());
-   * fields.put(fImpFileName, parser.getFields());
-   * allFields.put(fImpFileName, parser.getallFields());
-   * fieldsTable.put(fImpFileName, parser.getFieldsTable());
-   */
-
-  //  var ids: ArrayList[String] = new ArrayList[String]()
-  //  var associations: ArrayList[String] = null
-  //  var typeList: HashMap[String, String] = null
-  //  var sigs: ArrayList[Sig] = null
-  var intScope: Integer = 6
-
-  //	type ImplementationType = String
-  //  override type BenchmarkType = String
   type SpecificationType >: DBSpecification
   type ImplementationType >: DBImplementation
-  type MeasurementFunctionSetType >: DBBenchmark
   type FormalSpecificationType >: DBFormalSpecification
   type FormalImplementationType >: DBFormalImplementation
-  type FormalAbstractBenchmarkType >: DBFormalAbstractBenchmark
-  type FormalConcreteBenchmarkType >: DBFormalConcreteBenchmark
+
+  def run() = {
+    var isDebugOn = AppConfig.getDebug
+
+    var mySpec: DBSpecification = new DBSpecification(AppConfig.getSpecificationPath)
+    //    mySpec.setSpecFile("/Users/tang/Desktop/ORM/Parser/customerOrderObjectModel.als")
+
+    //    var myDBTrademaker = new DBTrademaker()
+    // get solutions and test results
+    var evaluatedResults = tradespaceFunction(mySpec)
+
+    // write the result to files and print it out
+    // iterate list of results
+    // get head of the list 
+    // get the tail of the list
+    var nilElem = Nil[Pair[ImplementationType, MeasurementFunctionSetType]]()
+    var defaultValue = Pair[ImplementationType, MeasurementResultSetType](new DBImplementation(""),
+      new DBMeasurementResult(new DBTimeMeasurementResult(-1.0, -1.0), new DBSpaceMeasurementResult(-1.0)));
+
+    var castedResults = evaluatedResults.asInstanceOf[List[Pair[ImplementationType, MeasurementResultSetType]]]
+    var resultHead = hd[Pair[ImplementationType, MeasurementResultSetType]](defaultValue)(castedResults)
+    var resultTail = tl[Pair[ImplementationType, MeasurementResultSetType]](castedResults)
+
+    if (resultHead != defaultValue) {
+      var implPath: String = fst(resultHead).asInstanceOf[DBImplementation].getImPath
+      var specName = implPath.substring(implPath.lastIndexOf(File.separator) + 1, implPath.indexOf("_"))
+      implPath = implPath.substring(0, implPath.lastIndexOf(File.separator))
+      implPath = implPath.substring(0, implPath.lastIndexOf(File.separator) + 1)
+      var resultFilePath = implPath + specName + ".txt"
+
+      //    var writeToFile = "/home/tang/Desktop/ORM/Parser/customerOrderObjectModel/"
+      var resultFile = new File(resultFilePath)
+      var pw = new PrintWriter(resultFile)
+
+      while (resultHead != defaultValue) {
+        var impl = fst(resultHead)
+        var mr = snd(resultHead)
+
+        var sol = impl.asInstanceOf[DBImplementation].getImPath
+        var solName = sol.substring(sol.lastIndexOf(File.separator) + 1, sol.lastIndexOf("."))
+        pw.println(solName + ":" + mr.asInstanceOf[DBMeasurementResult].getTmr().getInsertTime() + ":" +
+          mr.asInstanceOf[DBMeasurementResult].getTmr().getSelectTime() + ":" +
+          mr.asInstanceOf[DBMeasurementResult].getSmr().getDbSpace())
+
+        resultHead = hd[Pair[ImplementationType, MeasurementResultSetType]](defaultValue)(resultTail)
+        resultTail = tl[Pair[ImplementationType, MeasurementResultSetType]](resultTail)
+      }
+      pw.close()
+    }
+    if (isDebugOn) {
+      println("Done")
+    }
+  }
 
   def mySynthesizer(spec: SpecificationType): (List[Prod[ImplementationType, MeasurementFunctionSetType]]) = {
 
@@ -108,20 +127,25 @@ class DBTrademaker extends TrademakerFramework {
 
     var fImpl: List[FormalImplementationType] = myCFunction(fSpec)
 
-    var cImpl: List[ImplementationType] = myIFunctionHelper(fImpl)
+    //    var impls: List[ImplementationType] = myIFunctionHelper(fImpl)
+    var impls = myIFunctionHelper(fImpl)
 
     var fAbsMF: FormalAbstractMeasurementFunctionSet = myLFunction(fSpec)
 
-    var fConMF: List[FormalConcreteMeasurementFunctionSet] = myTFunction(fAbsMF)(cImpl)
+    var fConMF: List[FormalConcreteMeasurementFunctionSet] = myTFunction(fAbsMF)(impls)
 
-    var bms: List[MeasurementFunctionSetType] = myBFunctionHelper(fConMF)
+    //    var mfs: List[MeasurementFunctionSetType] = myBFunctionHelper(fConMF)
+    var mfs = myBFunctionHelper(fConMF)
 
-    var zipped = combine(cImpl)(bms)
+    var zipped = combine(impls)(mfs)
     zipped
   }
 
   def myRunBenchmark(prod: Prod[ImplementationType, MeasurementFunctionSetType]): Prod[ImplementationType, MeasurementResultSetType] = {
-    println("This is myRunBenchmark function")
+    if (isDebugOn) {
+      println("This is myRunBenchmark function")
+    }
+
     // impl = ... fst prod
     // tmf = ...
     // smf = ...
@@ -136,15 +160,17 @@ class DBTrademaker extends TrademakerFramework {
     tmf.setImpl(impl)
     var smf = mfs.getCsmf()
     smf.setImpl(impl)
-
-    println("=======================")
-    println("TimeMeasurementFunction")
-    println("=======================")
+    if (isDebugOn) {
+      println("=======================")
+      println("TimeMeasurementFunction")
+      println("=======================")
+    }
     var tmr = tmf.run()
-    println("=======================")
-    println("SpaceMeasurementFunction")
-    println("=======================")
-
+    if (isDebugOn) {
+      println("=======================")
+      println("SpaceMeasurementFunction")
+      println("=======================")
+    }
     var smr = smf.run()
 
     var dbmr = new DBMeasurementResult(tmr, smr)
@@ -165,7 +191,9 @@ class DBTrademaker extends TrademakerFramework {
    * Stub out ParetoFront
    */
   def myParetoFilter(list: List[Prod[ImplementationType, MeasurementResultSetType]]): List[Prod[ImplementationType, MeasurementResultSetType]] = {
-    println("This is myParetoFilter function")
+    if (isDebugOn) {
+      println("This is myParetoFilter function")
+    }
     Nil[Prod[ImplementationType, MeasurementResultSetType]]()
   }
 
@@ -180,8 +208,9 @@ class DBTrademaker extends TrademakerFramework {
    * Define functions for Trademaker in specification
    */
   def myCFunction(fSpec: FormalSpecificationType): List[FormalImplementationType] = {
-    println("This is myCFunction function")
-
+    if (isDebugOn) {
+      println("This is myCFunction function")
+    }
     /*
      * get specification file path
      * calculate solution folder based on specification file path
@@ -193,6 +222,7 @@ class DBTrademaker extends TrademakerFramework {
     var solFolder: String = specPath.substring(0, specPath.lastIndexOf("/"))
     var alloyOMName = specPath.substring(specPath.lastIndexOf("/") + 1, specPath.lastIndexOf("."))
     solFolder = solFolder + File.separator + alloyOMName + File.separator + "ImplSolution"
+    recursiveDelete(new File(solFolder))
     if (!new File(solFolder).exists()) {
       new File(solFolder).mkdirs()
     }
@@ -200,16 +230,13 @@ class DBTrademaker extends TrademakerFramework {
     // get mapping run file
     var mappingRun: String = FileOperation.getMappingRun(specPath)
     // call smartBridge
-    new SmartBridge(solFolder, mappingRun, 100000);
+    new SmartBridge(solFolder, mappingRun, AppConfig.getMaxSolForImpl);
     // delete mappingRun file
     new File(mappingRun).delete()
 
     // scan solution folder, and get all the solutions
     var solFiles: Array[File] = new java.io.File(solFolder).listFiles.filter(_.getName.endsWith(".xml"))
-    //     * var benchMarkFolder = solFolder+File.separator+"Benchmark"
     var imFile: File = null
-    //     * var insertBMFile:File = null
-    //     * var size:Integer = solFiles.length
     var implList: List[FormalImplementationType] = Nil[FormalImplementationType]()
 
     for (file <- solFiles) {
@@ -226,11 +253,13 @@ class DBTrademaker extends TrademakerFramework {
   }
 
   def myAFunction(fImp: FormalImplementationType): FormalSpecificationType = {
-    println("This is myAFunction function")
+    if (isDebugOn) {
+      println("This is myAFunction function")
+    }
     ""
   }
 
-  def myLFunction(fSpec: FormalSpecificationType): FormalAbstractMeasurementFunctionSet /*List[AbstractLoad]*/ = {
+  def myLFunction(fSpec: FormalSpecificationType): FormalAbstractMeasurementFunctionSet = {
     // generate two abstract load objects:  insert and select
     // create two measurement functions, one for time, one for space 
     // wrap them in a FormalAbstractMeasurementFunctionSet 
@@ -264,6 +293,8 @@ class DBTrademaker extends TrademakerFramework {
     var insAbsLoad = new AbstractLoad()
     var selAbsLoad = new AbstractLoad()
 
+    // random or synthesized abstract loads here
+
     // for each object solution to fSpec
     var objSpec = genObjSpec(fSpec)
 
@@ -271,15 +302,10 @@ class DBTrademaker extends TrademakerFramework {
     var specPath = objSpec.getSpecPath()
     var lenOfExtension = "_dm.als".length()
     var objectSolFolder = specPath.substring(0, specPath.length() - lenOfExtension)
-    //    var specName = specPath.substring(specPath.lastIndexOf(File.separator) + 1, specPath.indexOf("_"))
+
     objectSolFolder = objectSolFolder + File.separator + "TestSolutions"
     recursiveDelete(new File(objectSolFolder))
-    //        new File(objectSolFolder).delete()
     new File(objectSolFolder).mkdirs()
-    // create solution folder
-    //    if (!new File(objectSolFolder).exists()) {
-    //      new File(objectSolFolder).mkdirs()
-    //    }
 
     // call objects generator
     var loadSynthesizer = new LoadSynthesizer()
@@ -329,7 +355,11 @@ class DBTrademaker extends TrademakerFramework {
     var i: DBFormalImplementation = null
     var it = impls.iterator()
     while (it.hasNext()) {
-      returnValue.add(getConcreteMeasurementFunctionSet(absMF, it.next()))
+      var nextImpl = it.next()
+      if (isDebugOn) {
+        println("tFunction, for solution: " + nextImpl.asInstanceOf[DBImplementation].getImPath)
+      }
+      returnValue.add(getConcreteMeasurementFunctionSet(absMF, nextImpl))
     }
     returnValue
   }
@@ -363,6 +393,7 @@ class DBTrademaker extends TrademakerFramework {
       insertFile.createNewFile()
     }
     var insertPw: PrintWriter = new PrintWriter(insertFile)
+    insertPw.println("USE " + implFileName + ";")
     var allInsertStmts = new ArrayList[HashMap[String, HashMap[Integer, String]]]();
     var printOrder = PrintOrder.getOutPutOrders(pathBase)
     for (elem <- insCL.getQuerySet()) {
@@ -392,11 +423,16 @@ class DBTrademaker extends TrademakerFramework {
     // call shell command to remove duplicated lines,
     // and write results back to tmp.sql file
     var tmpFiles = pathBase + File.separator + "tmp.sql"
-    var strCmd = "awk '!x[$0]++' " + insertPath
-//    (Process(strCmd) #> new File(tmpFiles)).!
+    //    var strCmd = "awk '!x[$0]++' " + insertPath
+    //    (Process(strCmd) #> new File(tmpFiles)).!
+    // remove duplicate lines
     (Process(Seq("awk", "!x[$0]++", insertPath)) #> new File(tmpFiles)).!
+    var tmpFiles1 = tmpFiles + "1"
+    // add "FLUSH TABLES;" after each line
+    (Process(Seq("awk", "1;!(NR%1){print \"FLUSH TABLES;\";}", tmpFiles)) #> new File(tmpFiles1)).!
     // mv tmp file to insert file
-    Process(Seq("mv", tmpFiles, insertPath)).!
+    Process(Seq("mv", tmpFiles1, insertPath)).!
+    Process(Seq("rm", tmpFiles)).!
 
     // convert select statements
     var selCL = convert(selAL, impl)
@@ -410,6 +446,7 @@ class DBTrademaker extends TrademakerFramework {
       selectFile.createNewFile()
     }
     var selectPw: PrintWriter = new PrintWriter(selectFile)
+    selectPw.println("USE " + implFileName + ";")
     var allSelectStmts = new ArrayList[HashMap[String, ArrayList[String]]]();
     for (elem <- selCL.getQuerySet()) {
       var sq = elem.getSq()
@@ -435,11 +472,16 @@ class DBTrademaker extends TrademakerFramework {
     // call shell command to remove duplicated lines,
     // and write results back to tmp.sql file
     tmpFiles = pathBase + File.separator + "tmp.sql"
-    strCmd = "awk '!x[$0]++' " + selectPath
-//    (Process(strCmd) #> new File(tmpFiles)).!
-    (Process(Seq("awk", "!x[$0]++", selectPath)) #> new File(tmpFiles)).! 
+    //    strCmd = "awk '!x[$0]++' " + selectPath
+    //    (Process(strCmd) #> new File(tmpFiles)).!
+    //    remove duplicate lines
+    var tmpFiles2 = tmpFiles + "2"
+    (Process(Seq("awk", "!x[$0]++", selectPath)) #> new File(tmpFiles)).!
+    //    add "RESET QUERY CACHE;" after each line
+    (Process(Seq("awk", "1;!(NR%1){print \"RESET QUERY CACHE;\";}", tmpFiles)) #> new File(tmpFiles2)).!
     // mv tmp file to insert file
-    Process(Seq("mv", tmpFiles, selectPath)).!
+    Process(Seq("mv", tmpFiles2, selectPath)).!
+    Process(Seq("rm", tmpFiles)).!
 
     var ctmf: DBFormalConcreteTimeMeasurementFunction = new DBFormalConcreteTimeMeasurementFunction(insCL, selCL)
     concMFSet.setCtmf(ctmf)
@@ -524,11 +566,11 @@ class DBTrademaker extends TrademakerFramework {
     }
     insertPath += File.separator + implFileName + "_insert.sql"
 
-    while (it.hasNext) {
+    while (it.hasNext) { // iterate all instances in an object
       var instances = it.next
       var element: String = instances._1 // get key. tableName
       var instancesIt = instances._2.iterator
-      while (instancesIt.hasNext) {
+      while (instancesIt.hasNext) { // iterate all instances for one class
         var singleInstance = instancesIt.next
         var instanceName: String = singleInstance._1
         var fieldValuePairs = singleInstance._2
@@ -561,6 +603,10 @@ class DBTrademaker extends TrademakerFramework {
               } else {
                 var isFKey = isForeignKey(dbScheme, goToTable, fieldName)
                 if (isFKey) {
+                  // find association
+                  // find the foreign tables by primary key
+                  // this function may returns a list of tables, for example, customer ID is the
+                  // primary key of Customer table and also PreferredCustomer table
                   fTables = getTablesByPrimaryKey(impl.getPrimaryKeys, fieldName)
                   asss.clear()
                   for (fTable <- fTables) {
@@ -596,7 +642,7 @@ class DBTrademaker extends TrademakerFramework {
           field_part = field_part.substring(0, field_part.length() - 1)
           value_part = value_part.substring(0, value_part.length() - 1)
           var stmt: String = "INSERT INTO `" + goToTable + "` (" + field_part + ") VALUES (" + value_part + ");"
-          stmt += "FLUSH TABLES;";
+          //          stmt += "FLUSH TABLES;";
           // add statments
           if (!dataSchemaHasInsertStatement(allInsertStmts, goToTable, Integer.valueOf(id_value))) {
             addInsertStmtIntoDataSchema(allInsertStmts, goToTable, stmt, Integer.valueOf(id_value));
@@ -686,7 +732,7 @@ class DBTrademaker extends TrademakerFramework {
       for (pair <- entryValue) {
         if (pair.getFirst().split("_")(1).equalsIgnoreCase(srcDst1)) {
           var intValue: Integer = Integer.valueOf(pair.getSecond()).intValue();
-          var power = scala.math.pow(2, (intScope - 1))
+          var power = scala.math.pow(2, (AppConfig.getIntScopeForTestCases - 1))
           intValue = intValue + power.intValue() + 1;
           return String.valueOf(intValue)
         }
@@ -708,20 +754,19 @@ class DBTrademaker extends TrademakerFramework {
 
   def getFieldValue(fieldValues: ArrayList[CodeNamePair[String]], field: String): String = {
     var value: String = null
-    var pair: CodeNamePair[String] = null
     for (pair <- fieldValues) {
       if (pair.getFirst().split("_")(1).equalsIgnoreCase(field)) {
         var tmp: String = pair.getSecond();
         if (isNumeric(tmp)) {
           var intValue = Integer.valueOf(tmp).intValue()
-          var power = scala.math.pow(2, (intScope - 1))
+          var power = scala.math.pow(2, (AppConfig.getIntScopeForTestCases - 1))
           intValue = intValue + power.intValue() + 1
           value = String.valueOf(intValue)
           return value
         }
       }
     }
-    null
+    return value
   }
 
   def isNumeric(str: String): Boolean = {
@@ -733,7 +778,7 @@ class DBTrademaker extends TrademakerFramework {
 
   def getPrimaryKeyByTableName(dbScheme: HashMap[String, ArrayList[CodeNamePair[String]]], tableName: String): String = {
     var table: ArrayList[CodeNamePair[String]] = dbScheme.get(tableName);
-    var pair: CodeNamePair[String] = null
+    //    var pair: CodeNamePair[String] = null
     for (pair <- table) {
       if (pair.getFirst().equalsIgnoreCase("primaryKey")) {
         return pair.getSecond()
@@ -838,7 +883,7 @@ class DBTrademaker extends TrademakerFramework {
           wherePart = wherePart.substring(0, wherePart.length() - 5);
           var stmt = selectPart + fromPart + wherePart + ";";
           if (!stmt.substring(0, 11).equalsIgnoreCase("select from")) {
-            stmt += "RESET QUERY CACHE;";
+            //            stmt += "RESET QUERY CACHE;";
             addSelectStmtIntoDataSchema(allSelectStmts, goToTable, stmt);
           }
         }
@@ -857,6 +902,14 @@ class DBTrademaker extends TrademakerFramework {
     }
     allStmts.get(tableName).add(stmt)
   }
+  
+  /**
+   * This method will return  be called by 
+   */
+  def randomObjectsGenerator() : ObjectSet = {
+    null
+  }
+  
 
   def genObjects(objSpec: ObjectSpec): ObjectSet = {
     /**
@@ -873,6 +926,7 @@ class DBTrademaker extends TrademakerFramework {
     var objectSolFolder = specPath.substring(0, specPath.length() - lenOfExtension)
     //    var specName = specPath.substring(specPath.lastIndexOf(File.separator) + 1, specPath.indexOf("_"))
     objectSolFolder = objectSolFolder + File.separator + "TestSolutions"
+    recursiveDelete(new File(objectSolFolder))
     if (!new File(objectSolFolder).exists()) {
       new File(objectSolFolder).mkdirs()
     }
@@ -895,7 +949,9 @@ class DBTrademaker extends TrademakerFramework {
   }
 
   def genObjSpec(fSpec: FormalSpecificationType): ObjectSpec = {
-    println("This is myLFunction function")
+    if (isDebugOn) {
+      println("This is myLFunction function")
+    }
     /**
      * construct object specification name from FormalSpecification
      * manually set intScopt as 6 (task)
@@ -904,11 +960,10 @@ class DBTrademaker extends TrademakerFramework {
      */
     var fSpecPath = fSpec.asInstanceOf[DBFormalSpecification].getSpec
     var objSpecPath = fSpecPath.substring(0, fSpecPath.length() - 4) + "_dm.als"
-    var intScope = 6
 
     var aotad: AlloyOMToAlloyDM = new AlloyOMToAlloyDM()
     // by calling run, (legacy) Object Specification will be created
-    aotad.run(fSpecPath, objSpecPath, intScope)
+    aotad.run(fSpecPath, objSpecPath, AppConfig.getIntScopeForTestCases)
 
     var objSpec = new ObjectSpec()
 
@@ -923,7 +978,9 @@ class DBTrademaker extends TrademakerFramework {
   }
 
   def myTFunction(fAB: FormalAbstractMeasurementFunctionSet): (List[ImplementationType] => List[FormalConcreteMeasurementFunctionSet]) = {
-    println("This is myTFunction function")
+    if (isDebugOn) {
+      println("This is myTFunction function")
+    }
     def returnFunction(implList: List[ImplementationType]): List[FormalConcreteMeasurementFunctionSet] = {
       // convert between List in extracted code and ArrayList in Java
       var impls: ArrayList[DBImplementation] = new ArrayList[DBImplementation]()
@@ -961,7 +1018,9 @@ class DBTrademaker extends TrademakerFramework {
   }
 
   def mySFunction(spec: SpecificationType): FormalSpecificationType = {
-    println("This is mySFunction function")
+    if (isDebugOn) {
+      println("This is mySFunction function")
+    }
     var dbfs = new DBFormalSpecification(spec.asInstanceOf[DBSpecification].getSpecFile)
     // parse spec file and fill in all members
     // Chong: check how to define constructor in Scala, and call parseSepc() in consctructor
@@ -986,8 +1045,9 @@ class DBTrademaker extends TrademakerFramework {
   }
 
   def myIFunction(fImp: FormalImplementationType): ImplementationType = {
-    println("This is myIFunction function")
-
+    if (isDebugOn) {
+      println("This is myIFunction function")
+    }
     /**
      * compute FormalImplementation schema name
      * sigs here is all signatures in FormalSpecification (alloyOM), which already be set by lFunction
