src/edu/virginia/cs/Main.scala
@@ -1,7 +1,7 @@
 package edu.virginia.cs
 
-import edu.virginia.cs.Framework._
-import edu.virginia.cs.Framework.TrademakerFramework
+import edu.virginia.cs.Framework.Types.DBSpecification
+import com.typesafe.config.ConfigFactory
 
 /**
  * @author tang
@@ -9,28 +9,25 @@ import edu.virginia.cs.Framework.TrademakerFramework
 
 // This is the Main class, the entry point of the DB instance of Trademaker Framework
 object Main {
-//  type SpecificationType >: edu.virginia.cs.Framework.SpecificationType
-//  type ImplementationType >: edu.virginia.cs.Framework.ImplementationType
-//  type BenchmarkType >: DBBenchmark
+  var isDebugOn = AppConfig.getDebug
   def main(args: Array[String]) {
-    var mySpec: DBSpecification = new DBSpecification()
-//    mySpec.setSpecFile("/Users/tang/Desktop/ORM/Parser/customerOrderObjectModel.als")
-    mySpec.setSpecFile("/home/tang/Desktop/ORM/Parser/customerOrderObjectModel.als")
-    //  
-    //  var myDBTradespace = new DBTradespace()
-    //  myDBTradespace.mySpec = ""
-    //  var evaluatedResults = myDBTradespace.tradespaceFunction(myDBTradespace.mySpec)
-    //  
-    //  var myDBParetoFront = new DBParetoFront()
-    //  var paretoSols = myDBParetoFront.getParetoResults(myDBTradespace.myTradespace, mySpec.getSpecFile)
-    //  
-    ////  var paretoFront = myParetoFront.paretoFront(myParetoFront)
+
+    var mySpec: DBSpecification = new DBSpecification(AppConfig.getSpecificationPath)
+    //    mySpec.setSpecFile("/Users/tang/Desktop/ORM/Parser/customerOrderObjectModel.als")
 
     var myDBTrademaker = new DBTrademaker()
     // get solutions and test results
-    var evaluatedResults = myDBTrademaker.tradespaceFunction(mySpec)
-
-    println("Done")
+//    var evaluatedResults = myDBTrademaker.tradespaceFunction(mySpec)
+    myDBTrademaker.run()
+    // write the result to files and print it out
+    // iterate list of results
+    // get head of the list 
+    // get the tail of the list
+    
+//    var tmpPair = Pair[ImplementationType, MeasurementFunctionSetType]()
+    
+    if (isDebugOn) {
+      println("Done")
+    }
   }
-
 }
