CoqSpec/CoqTypeClasses.v
@@ -3,18 +3,37 @@ Require Import String.
 
 Open Scope list_scope.
 
-
 Class Tradespace := {
     SpecificationType: Set
   ; ImplementationType: Set
   ; MeasurementFunctionSetType: Set
   ; MeasurementResultSetType: Set
-  ; synthesize: SpecificationType -> list (ImplementationType * MeasurementFunctionSetType)
+  ; synthesize : SpecificationType -> list (ImplementationType * MeasurementFunctionSetType)
   ; runBenchmark: ImplementationType * MeasurementFunctionSetType -> (ImplementationType * MeasurementResultSetType)
   ; analyze (input: list (ImplementationType * MeasurementFunctionSetType)) : list (ImplementationType * MeasurementResultSetType) :=
       map runBenchmark input
   ; tradespace (spec: SpecificationType): list (ImplementationType * MeasurementResultSetType) :=
      analyze (synthesize spec) 
+}.
+
+Inductive DBSpecification: Set := DBSpecification1.
+Inductive DBImplementation: Set := DBImplementation1.
+Inductive DBMeasurementFunctionSet: Set := DBMeasurementFunctionSet1.
+Inductive DBMeasurementResultSet: Set :=  DBMeasurementResultSet1.
+
+Definition dbSynthesize (spec: DBSpecification) : list (DBImplementation * DBMeasurementFunctionSet) :=
+  (DBImplementation1, DBMeasurementFunctionSet1) :: nil.
+
+Definition dbRunBenchmark (mfPair : DBImplementation * DBMeasurementFunctionSet) : (prod DBImplementation DBMeasurementResultSet) := 
+  (DBImplementation1, DBMeasurementResultSet1).
+
+Instance DBTradeSpace: Tradespace := {
+   SpecificationType := DBSpecification
+  ; ImplementationType := DBImplementation
+  ; MeasurementFunctionSetType := DBMeasurementFunctionSet
+  ; MeasurementResultSetType := DBMeasurementResultSet
+  ; synthesize := dbSynthesize
+  ; runBenchmark := dbRunBenchmark
 }.
 
 
@@ -24,6 +43,15 @@ Class ParetoFront := {
   ; paretoFront (spec: SpecificationType): list (ImplementationType * MeasurementResultSetType) := paretoFilter (tradespace spec)
 }.
 
+Definition DBParetoFilter (implList: list (DBImplementation * DBMeasurementResultSet)) := 
+  (DBImplementation1, DBMeasurementResultSet1) :: nil.
+
+Instance DBParetoFront: ParetoFront := {
+    pf_tradespace := DBTradeSpace
+  ; paretoFilter := DBParetoFilter
+}.
+
+
 Class Trademaker := {
     tm_Tradespace :> Tradespace
   ; tm_ParetoFront :> ParetoFront
@@ -31,36 +59,87 @@ Class Trademaker := {
   (* Internal, formal-specification-based types *)
   ; FormalSpecificationType: Set
   ; FormalImplementationType: Set
-  ; FormalAbstractMeasurementFunctionSet: Set
-  ; FormalConcreteMeasurementFunctionSet: Set
+  ; FormalAbstractMeasurementFunctionSetType: Set
+  ; FormalConcreteMeasurementFunctionSetType: Set
 
   (* Internal, formal-specification-based functions *)
   ; cFunction: FormalSpecificationType -> list FormalImplementationType
   ; aFunction: FormalImplementationType -> FormalSpecificationType
-  ; lFunction: FormalSpecificationType -> FormalAbstractMeasurementFunctionSet
-  ; tFunction: FormalAbstractMeasurementFunctionSet -> list FormalImplementationType -> list FormalConcreteMeasurementFunctionSet
+  ; lFunction: FormalSpecificationType -> FormalAbstractMeasurementFunctionSetType
+  ; tFunction: FormalAbstractMeasurementFunctionSetType -> list ImplementationType -> list FormalConcreteMeasurementFunctionSetType
 
   (* mappings into and out of formal-specification-based representations *)
   ; sFunction: SpecificationType -> FormalSpecificationType
   ; iFunction: FormalImplementationType -> ImplementationType
-  ; bFunction: FormalConcreteMeasurementFunctionSet -> MeasurementFunctionSetType
+  ; bFunction: FormalConcreteMeasurementFunctionSetType -> MeasurementFunctionSetType
 
   (* Laws *)
-  ; aInvertsC: forall (spec: FormalSpecificationType) (impl: FormalImplementationType), In impl (cFunction spec) -> (spec = aFunction impl)
+  ; aInvertsC: forall (spec: FormalSpecificationType) (fImpl: FormalImplementationType), In fImpl (cFunction spec) -> (spec = aFunction fImpl)
 
-  ; implementationLine: forall (spec: SpecificationType) (cdt: FormalImplementationType) (impl: ImplementationType) (bmt: MeasurementFunctionSetType) 
-                          (clt: FormalConcreteMeasurementFunctionSet) (adt: FormalSpecificationType) (alt: FormalAbstractMeasurementFunctionSet), 
-                            (adt = sFunction spec) 
-                              -> (In cdt (cFunction adt)) 
-                                -> (impl = iFunction cdt) -> In impl (map (@fst ImplementationType  MeasurementFunctionSetType) (synthesize spec)) 
+  ; implementationLine: forall (spec: SpecificationType) (fImpl: FormalImplementationType) (impl: ImplementationType) (fSpec: FormalSpecificationType), 
+                            (fSpec = sFunction spec) -> (In fImpl (cFunction fSpec)) -> (impl = iFunction fImpl) 
+                                           -> In impl (map (@fst ImplementationType  MeasurementFunctionSetType) (synthesize spec)) 
 
-  ; testLoadsLine: forall (st: SpecificationType) (cdt: FormalImplementationType) (imt: ImplementationType) (bmt: MeasurementFunctionSetType) 
-                          (clt: FormalConcreteMeasurementFunctionSet) (adt: FormalSpecificationType) (alt: FormalAbstractMeasurementFunctionSet), 
-                           (adt = sFunction st) -> (alt = (lFunction adt)) -> (In clt (tFunction alt (cFunction adt)))
-                            -> (bmt = bFunction clt) -> In bmt (map (@snd ImplementationType  MeasurementFunctionSetType) (synthesize st))
+  ; testLoadsLine: forall (spec: SpecificationType) (mfs: MeasurementFunctionSetType) (fCMFs: FormalConcreteMeasurementFunctionSetType)
+                          (fSpec: FormalSpecificationType) (fAMFs: FormalAbstractMeasurementFunctionSetType) (impl: ImplementationType)
+                          (fImpl: FormalImplementationType),
+                          (fSpec = sFunction spec) -> (In fImpl (cFunction fSpec)) -> (fAMFs = (lFunction fSpec)) ->
+                          (In fCMFs (tFunction  fAMFs (map iFunction (cFunction fSpec)))) -> (mfs = bFunction fCMFs) -> 
+                          In mfs (map (@snd ImplementationType  MeasurementFunctionSetType) (synthesize spec))
 }.
 
 
+Inductive DBFormalSpecification: Set := DBFormalSpecification1.
+Inductive DBFormalImplementation: Set := DBFormalImplementation1.
+Inductive DBFormalAbstractMeasurementFunctionSet: Set := DBFormalAbstractMeasurementFunctionSet1.
+Inductive DBFormalConcreteMeasurementFunctionSet: Set := DBFormalConcreteMeasurementFunctionSet1.
+
+Definition dbCFunction (spec: DBFormalSpecification) : list DBFormalImplementation := 
+  DBFormalImplementation1::nil.
+
+Definition dbAFunction (impl: DBFormalImplementation) : DBFormalSpecification := DBFormalSpecification1.
+
+Definition dbLFunction (spec: DBFormalSpecification) : DBFormalAbstractMeasurementFunctionSet := DBFormalAbstractMeasurementFunctionSet1.
+
+Definition dbTFunction (dbFAMFS: DBFormalAbstractMeasurementFunctionSet) (implList: list ImplementationType) : list DBFormalConcreteMeasurementFunctionSet := 
+  DBFormalConcreteMeasurementFunctionSet1::nil.
+
+Definition dbSFunction (spec: DBSpecification) : DBFormalSpecification := DBFormalSpecification1.
+Definition dbIFunction (fImpl: DBFormalImplementation) : DBImplementation := DBImplementation1.
+Definition dbBFunction (dbFCMFS: DBFormalConcreteMeasurementFunctionSet) : DBMeasurementFunctionSet := DBMeasurementFunctionSet1.
+
+Instance DBTrademaker : Trademaker := {
+    tm_Tradespace := DBTradeSpace
+  ; tm_ParetoFront := DBParetoFront
+  ; FormalSpecificationType := DBFormalSpecification
+  ; FormalImplementationType := DBFormalImplementation
+  ; FormalAbstractMeasurementFunctionSetType := DBFormalAbstractMeasurementFunctionSet
+  ; FormalConcreteMeasurementFunctionSetType := DBFormalConcreteMeasurementFunctionSet
+  ; cFunction := dbCFunction
+  ; aFunction := dbAFunction
+  ; lFunction := dbLFunction
+  ; tFunction := dbTFunction
+  ; sFunction := dbSFunction
+  ; iFunction := dbIFunction
+  ; bFunction := dbBFunction
+}.
+Proof.
+intros.
+induction fImpl.
+induction spec.
+compute. reflexivity.
+intros.
+induction spec.
+compute.
+induction impl.
+apply or_introl. reflexivity.
+intros.
+induction spec.
+compute.
+apply or_introl.
+induction mfs.
+reflexivity.
+Qed.
 
 Extraction Language Scala.
 Recursive Extraction 
@@ -70,8 +149,8 @@ MeasurementFunctionSetType
 MeasurementResultSetType
 FormalSpecificationType
 FormalImplementationType
-FormalAbstractMeasurementFunctionSet
-FormalConcreteMeasurementFunctionSet
+FormalAbstractMeasurementFunctionSetType
+FormalConcreteMeasurementFunctionSetType
 synthesize
 runBenchmark
 analyze
